ADTExamples/QueryStructure/InsertQSSpecs.v
@@ -1,0 +1,42 @@
+Require Import List String Ensembles
+        ADTNotation Program QueryStructureSchema QueryStructure.
+
+(* Definitions for updating query structures. *)
+
+Definition QSInsertSpec
+           {QSSchema}
+           (qs : QueryStructure QSSchema)
+           (idx : qschemaIndex QSSchema)
+           (tup : Tuple (schemaHeading (qschemaSchema _ idx)))
+           (qs' : QueryStructure QSSchema)
+: Prop :=
+  (* All of the relations with a different index are untouched
+     by insert. *)
+  (forall idx' (rel : Relation (qschemaSchema QSSchema idx')),
+     idx <> idx' ->
+     rels qs idx' rel <-> rels qs' idx' rel) /\
+  (* If [tup] is consistent with the schema constraints and the
+     cross-relation constraints, it is included in the relation
+     indexed by [idx] after insert; that relation is unspecified if
+     [tup] does not satisfy either set of constraints. *)
+  schemaConstraints (qschemaSchema QSSchema idx) tup
+  -> (forall idx' (rel' : Relation (qschemaSchema QSSchema idx')),
+        rels qs idx' rel'
+        -> qschemaConstraints QSSchema idx idx' tup rel')
+  -> forall (tup' : Tuple (schemaHeading (qschemaSchema _ idx)))
+            (rel' : Relation (qschemaSchema QSSchema idx)),
+       rels qs' idx rel' ->
+       (* A tuple [tup'] included in the modified relation [rel']
+          iff it is equal to [tup] or it was included in the original
+          relation [rel]. *)
+       (rel rel' tup' ->
+        tup = tup' \/
+        exists rel'' : Relation (qschemaSchema QSSchema idx),
+          rels qs idx rel'' /\ rel rel'' tup') /\
+       (tup = tup' -> rel rel' tup') /\
+       (forall rel'' : Relation (qschemaSchema QSSchema idx),
+          rels qs idx rel'' -> rel rel'' tup' -> rel rel' tup').
+
+Notation "'Insert' b 'into' idx 'of' r " :=
+  (QSInsertSpec r {| bstring := idx%string |} b)
+    (at level 80) : QuerySpec_scope.
