ADTExamples/QueryStructure/QueryQSSpecs.v
@@ -1,0 +1,35 @@
+Require Import List String Ensembles
+        ADTNotation Program QueryStructureSchema QueryStructure.
+
+(* Notations for queries. *)
+
+(* This typeclass allows our 'in' notation to avoid
+   mentioning the QueryStructure. *)
+
+Class QueryStructureHint :=
+  { qsSchemaHint : QueryStructureSchema;
+     qsHint :> @QueryStructure qsSchemaHint
+  }.
+
+Notation "( x 'in' R ) bod" :=
+  (fun bx =>
+     exists r x, R%QueryStructure r /\
+                 rel r x /\
+                 (bod bx)%QuerySpec) : QuerySpec_scope.
+
+Notation "'Return' t" :=
+  (fun rx => rx = t%Tuple) : QuerySpec_scope.
+
+Notation "'Where' p bod" :=
+  (fun wx => p%Tuple /\ (bod wx)%QuerySpec) : QuerySpec_scope.
+
+Notation "'For' bod 'returning' sch" :=
+  (@Build_Relation
+    sch bod%QuerySpec (fun _ _ => I))
+  : QuerySpec_scope.
+
+(* The spec for a count of the number of tuples in a relation.  *)
+Definition Count {Schema} (R : Relation Schema) (n : nat) :=
+  forall tup l,
+    (List.In tup l <-> rel R tup) <->
+    n = List.length l.
