ADTExamples/QueryStructure/Notations.v
@@ -5,6 +5,9 @@ Reserved Notation "< col1 , .. , coln >"
          (at level 0, col1, coln at level 60,
           format "< '[v  ' col1 ,  .. ,  coln ']' >").
 
+Reserved Notation "t ''s' R"
+         (at level 70, format "t ''s' R").
+
 Reserved Notation "'attributes' attrlist1 'depend' 'on' attrlist2 "
          (at level 50).
 
@@ -26,6 +29,22 @@ Reserved Notation "'query' 'structure' 'schema' relList "
 Reserved Notation "'query' 'structure' 'schema' relList 'enforcing' constraints"
          (at level 0, constraints at level 50).
 
+Reserved Notation "( x 'in' r ) bod"
+         (right associativity, at level 0,
+          format "( x  'in'  r ) '//' bod ").
+
+Reserved Notation "'Return' t"
+         (right associativity, at level 0,
+          format "'Return'  t" ).
+
+Reserved Notation "'Where' p bod"
+         (right associativity, at level 0, x at level 0, p at level 0,
+          format "'Where'  p '//' bod " ).
+
+Reserved Notation "'For' bod 'returning' sch"
+         (right associativity, at level 0,
+          format "'For'  '[v' bod ']' '//' 'returning'  sch").
+
 Delimit Scope Attribute_scope with Attribute.
 Delimit Scope Heading_scope with Heading.
 Delimit Scope Component_scope with Component.
@@ -36,3 +55,5 @@ Delimit Scope Schema_scope with Schema.
 Delimit Scope NamedSchema_scope with NamedSchema.
 Delimit Scope QSSchema_scope with QSSchema.
 Delimit Scope QSSchemaConstraints_scope with QSSchemaConstraints.
+Delimit Scope QuerySpec_scope with QuerySpec.
+Delimit Scope QueryStructure_scope with QueryStructure.
